PesudoElimination Finished

x86/PseudoInstructions.v
@@ -32,121 +32,15 @@ Definition transf_instr (i: instruction): list instruction :=
 Definition transf_code (c: code) : code :=
   concat (map transf_instr c).
 
-Section INSTRSIZE.
-Variable instr_size : instruction -> Z.
 Definition transf_function (f: function) :=
-  if   wf_asm_function_check instr_size f && AsmFacts.check_asm_code_no_rsp (fn_code f) then OK
   {|
     fn_sig := fn_sig f;
     fn_code := transf_code (fn_code f);
     fn_stacksize := fn_stacksize f;
     fn_ofs_link := fn_ofs_link f;
-  |}
-  else Error (MSG"Precondition of pseudo instruction elimination fails" ::nil).
+  |}.
 
-Definition transf_fundef := AST.transf_partial_fundef transf_function.
+Definition transf_fundef := AST.transf_fundef transf_function.
 
-Definition transf_program (p: Asm.program) : res Asm.program :=
-  AST.transform_partial_program transf_fundef p.
-
-End INSTRSIZE.
-(*
-Definition check_function (f: Asm.function) : bool :=
-  wf_asm_function_check f && AsmFacts.check_asm_code_no_rsp (fn_code f).
-
-Definition transf_check_function f :=
-  if check_function f then OK f
-  else Error (MSG "Precondition of pseudo instruction elimination fails" :: nil).
-
-Definition transf_check_fundef :=
-  AST.transf_partial_fundef (transf_check_function).
-
-Require Import Globalenvs.
-
-(* Definition has_main (p: program) := *)
-(*   let ge := Genv.globalenv p in *)
-(*   match Genv.find_symbol ge (prog_main p) with *)
-(*   | Some b => *)
-(*     match Genv.find_funct_ptr ge b with *)
-(*     | Some (Internal f) => true *)
-(*     | _ => false *)
-(*     end *)
-(*   | _ => false *)
-(*   end. *)
-
-Definition check_program p : res (Asm.program) :=
-  (* if has_main p *)
-  (* then *) AST.transform_partial_program transf_check_fundef p
-  (* else Error (msg "no main function in program") *).
-
-Theorem check_program_id:
-  forall p1 p2,
-    check_program p1 = OK p2 -> p1 = p2.
-Proof.
-  unfold check_program.
-  unfold transform_partial_program.
-  unfold transform_partial_program2.
-  intros. monadInv H. destruct p1. simpl in *. f_equal.
-  revert EQ.
-  unfold transf_check_fundef, transf_partial_fundef, transf_check_function.
-  revert x; induction prog_defs; simpl; intros; eauto. inv EQ; auto.
-  destr_in EQ.
-  repeat destr_in EQ; repeat destr_in Heqr; monadInv H0.
-  - f_equal. eauto.
-  - f_equal. eauto.
-  - f_equal; eauto. f_equal. f_equal. f_equal. destruct v; simpl. f_equal.
-  - f_equal. eauto.
-Qed.
-
-Definition match_check_prog (p: Asm.program) (tp: Asm.program) :=
-  Linking.match_program (fun _ f tf => transf_check_fundef f = OK tf) eq p tp (* /\ *)
-  (* exists (bmain : Values.block) (fmain : Asm.function), *)
-  (*   Globalenvs.Genv.find_symbol (Globalenvs.Genv.globalenv p) (prog_main p) = Some bmain /\ *)
-  (*   Globalenvs.Genv.find_funct_ptr (Globalenvs.Genv.globalenv p) bmain = Some (Internal fmain) *).
-
-Lemma check_program_match:
-  forall p tp, check_program p = OK tp -> match_check_prog p tp.
-Proof.
-  intros. unfold check_program in H. destr_in H.
-  eapply Linking.match_transform_partial_program; eauto.
-Qed.
-
-Theorem check_wf:
-  forall p tp,
-    match_check_prog p tp ->
-    RealAsm.wf_asm_prog (Globalenvs.Genv.globalenv p).
-Proof.
-  red.
-  intros.
-  destruct H as (A & B & C).
-  eapply Globalenvs.Genv.find_funct_ptr_prop with (P := fun f => match f with Internal f => _ f | _ => True end) in H0.
-  apply H0.
-  intros. edestruct list_forall2_in_left as (v2 & IN2 & P2); eauto.
-  inv P2. simpl in *. subst. inv H2. inv H4.
-  destr. simpl in H5. monadInv H5.
-  unfold transf_check_function in EQ. repeat destr_in EQ.
-  unfold check_function in Heqb0.
-  apply andb_true_iff in Heqb0; destruct Heqb0.
-  eapply wf_asm_function_check_correct; eauto.
-Qed.
-
-Theorem check_no_rsp:
-  forall p tp,
-    match_check_prog p tp ->
-    forall b f,
-      Globalenvs.Genv.find_funct_ptr (Globalenvs.Genv.globalenv p) b = Some (Internal f) ->
-      AsmFacts.check_asm_code_no_rsp (fn_code f) = true.
-Proof.
-  intros.
-  destruct H as (A & B & C).
-  eapply Globalenvs.Genv.find_funct_ptr_prop with (P := fun f => match f with Internal f => _ f | _ => True end) in H0.
-  pattern f.
-  apply H0.
-  simpl. intros. edestruct list_forall2_in_left as (v2 & IN2 & P2); eauto.
-  inv P2. simpl in *. subst. inv H2. inv H4.
-  destr. simpl in H5. monadInv H5.
-  unfold transf_check_function in EQ. repeat destr_in EQ.
-  unfold check_function in Heqb0.
-  apply andb_true_iff in Heqb0; destruct Heqb0; auto.
-Qed.
-*)
+Definition transf_program (p: Asm.program) : Asm.program :=
+  AST.transform_program transf_fundef p.
